src/lang/Progress.v
@@ -7,6 +7,7 @@ Require Import paco.
 Require Import Axioms.
 Require Import Basic.
 Require Import DataStructure.
+Require Import DenseOrder.
 Require Import Event.
 Require Import Time.
 Require Import Language.
@@ -17,6 +18,25 @@ Require Import Thread.
 Set Implicit Arguments.
 
 
+Lemma write_step_promise
+      lc1 mem1 loc from to val releasedc releasedm ord lc2 mem2
+      (STEP: Local.write_step lc1 mem1 loc from to val releasedc releasedm ord lc2 mem2)
+      (PROMISES: lc1.(Local.promises) = Memory.bot):
+  lc2.(Local.promises) = Memory.bot.
+Proof.
+  inv STEP.
+  - apply Memory.ext. i. rewrite Memory.bot_get.
+    destruct (Memory.get loc0 ts (Local.promises lc2)) as [[]|] eqn:X; auto.
+    inv FULFILL. ss. inv FULFILL0. eapply Memory.remove_get_inv in X; eauto. des.
+    rewrite PROMISES, Memory.bot_get in *. congr.
+  - apply Memory.ext. i. rewrite Memory.bot_get.
+    destruct (Memory.get loc0 ts (Local.promises lc2)) as [[]|] eqn:X; auto.
+    inv FULFILL. ss. inv FULFILL0. eapply Memory.remove_get_inv in X; eauto. des.
+    inv PROMISE. ss. eapply Memory.promise_promises_get2 in X0; eauto. des.
+    + subst. contradict X. auto.
+    + rewrite PROMISES, Memory.bot_get in *. congr.
+Qed.
+
 Lemma program_step_promise
       lang
       e st1 lc1 mem1 st2 lc2 mem2
@@ -24,26 +44,29 @@ Lemma program_step_promise
       (PROMISES: lc1.(Local.promises) = Memory.bot):
   lc2.(Local.promises) = Memory.bot.
 Proof.
-  inv STEP; try inv LOCAL; ss.
-  - admit.
-  - admit.
-  - admit.
-Admitted.
+  inv STEP; try by inv LOCAL.
+  - eapply write_step_promise; eauto.
+  - eapply write_step_promise; eauto.
+    inv LOCAL1. auto.
+Qed.
 
+Definition max_ts (loc:Loc.t) (mem:Memory.t): Time.t :=
+  DOMap.max_key _ (mem loc).(Cell.raw).
 
-Inductive max_timestamp (loc:Loc.t) (to:Time.t) (mem:Memory.t): Prop :=
-| max_timestamp_intro
-    from msg
-    (MSG: Memory.get loc to mem = Some (from, msg))
-    (MAX: forall to' (LT: Time.lt to to'), Memory.get loc to' mem = None)
-.
-
-Lemma exists_max_timestamp
+Lemma max_ts_spec
       loc mem
-      (WF: Memory.closed mem):
-  exists ts, max_timestamp loc ts mem.
+      (CLOSED: Memory.closed mem):
+  <<GET: exists from msg, Memory.get loc (max_ts loc mem) mem = Some (from, msg)>> /\
+  <<MAX: forall ts (GET: Memory.get loc ts mem <> None), Time.le ts (max_ts loc mem)>>.
 Proof.
-Admitted.
+  exploit (DOMap.max_key_spec _ (mem loc).(Cell.raw)); eauto.
+  { apply CLOSED. }
+  i. des. splits; eauto.
+  destruct (DOMap.find
+              (DOMap.max_key (DenseOrder.t * Message.t)
+              (Cell.raw (mem loc))) (Cell.raw (mem loc))) as [[]|] eqn:X; [|congr].
+  eexists _, _. eauto.
+Qed.
 
 (* TODO: `released` should be somehow constraint.
  * Note that we do not use `released_min`, since the update rule has `releasedr` components.
@@ -54,13 +77,12 @@ Admitted.
  *)
 Lemma progress_promise_step
       lc1 mem1
-      loc from to released val
-      (MAX: max_timestamp loc from mem1)
-      (LT: Time.lt from to)
+      loc to released val
+      (LT: Time.lt (max_ts loc mem1) to)
       (WF1: Local.wf lc1 mem1)
       (MEM1: Memory.closed mem1):
   exists promises2 mem2,
-    Local.promise_step lc1 mem1 loc from to val released (Local.mk lc1.(Local.commit) promises2) mem2.
+    Local.promise_step lc1 mem1 loc (max_ts loc mem1) to val released (Local.mk lc1.(Local.commit) promises2) mem2.
 Proof.
   destruct lc1. s.
   eexists _, _. econs.
@@ -80,22 +102,22 @@ Qed.
 
 Lemma progress_read_step
       lc1 mem1
-      loc ord ts
+      loc ord
       (WF1: Local.wf lc1 mem1)
       (MEM1: Memory.closed mem1)
-      (PROMISES1: lc1.(Local.promises) = Memory.bot)
-      (MAX: max_timestamp loc ts mem1):
+      (PROMISES1: lc1.(Local.promises) = Memory.bot):
   exists val released lc2,
-    Local.read_step lc1 mem1 loc ts val released ord lc2.
+    Local.read_step lc1 mem1 loc (max_ts loc mem1) val released ord lc2.
 Proof.
-  inv MAX. destruct msg.
-  exploit (@CommitFacts.read_min_spec loc ts released); try apply WF1; i.
-  { admit. }
-  { admit. }
-  { exploit MEM1; eauto. i. des. auto. }
+  exploit (max_ts_spec loc); eauto. i. des. destruct msg.
+  exploit (@CommitFacts.read_min_spec loc (max_ts loc mem1) released); try apply WF1; i.
+  { eapply MAX. inv WF1. inv COMMIT_CLOSED. inv CUR. exploit UR; eauto. i. des. rewrite x. congr. }
+  { eapply MAX. inv WF1. inv COMMIT_CLOSED. inv CUR. exploit RW; eauto. i. des. rewrite x. congr. }
+  { inv MEM1. exploit CLOSED; eauto. i. des. auto. }
   eexists _, _, _. econs; try apply x0; eauto.
-  admit. (* commit.closed *)
-Admitted.
+  eapply CommitFacts.read_min_closed; eauto.
+  apply WF1.
+Qed.
 
 Lemma progress_fulfill_step
       lc1 mem1
@@ -124,14 +146,13 @@ Admitted.
 
 Lemma progress_write_step
       lc1 mem1
-      loc from to val releasedc releasedm ord
-      (MAX: max_timestamp loc from mem1)
-      (LT: Time.lt from to)
+      loc to val releasedc releasedm ord
+      (LT: Time.lt (max_ts loc mem1) to)
       (WF1: Local.wf lc1 mem1)
       (MEM1: Memory.closed mem1)
       (PROMISES1: lc1.(Local.promises) = Memory.bot):
   exists lc2 mem2,
-    Local.write_step lc1 mem1 loc from to val releasedc releasedm ord lc2 mem2.
+    Local.write_step lc1 mem1 loc (max_ts loc mem1) to val releasedc releasedm ord lc2 mem2.
 Proof.
   destruct lc1. ss. subst.
   exploit progress_promise_step; eauto. s. i. des.
@@ -157,7 +178,9 @@ Lemma progress_fence_step
     Local.fence_step lc1 mem1 ordr ordw lc2.
 Proof.
   exploit CommitFacts.read_fence_min_spec; try apply WF1; eauto. i. des.
-  exploit CommitFacts.write_fence_min_spec; try apply WF; try apply WF1; eauto. i. des.
+  exploit CommitFacts.write_fence_min_spec; try apply x0. i.
   eexists. econs; eauto.
-  admit. (* commit.closed *)
-Admitted.
+  apply CommitFacts.write_fence_min_closed; eauto.
+  apply CommitFacts.read_fence_min_closed; eauto.
+  apply WF1.
+Qed.
