src/lang/Thread.v
@@ -63,7 +63,6 @@ Module Local.
       (PROMISES: lc.(promises) = Memory.bot)
   .
 
-  (* TODO: is it "right" to have the closedness of the memory here? *)
   Inductive wf (lc:t) (mem:Memory.t): Prop :=
   | wf_intro
       (COMMIT_WF: Commit.wf lc.(commit))
@@ -175,9 +174,9 @@ Module Local.
   Lemma promise_step_future lc1 mem1 loc from to val released lc2 mem2
         (STEP: promise_step lc1 mem1 loc from to val released lc2 mem2)
         (WF1: wf lc1 mem1)
-        (MEM1: Memory.closed mem1):
+        (CLOSED1: Memory.closed mem1):
     <<WF2: wf lc2 mem2>> /\
-    <<MEM2: Memory.closed mem2>> /\
+    <<CLOSED2: Memory.closed mem2>> /\
     <<FUTURE: Memory.future mem1 mem2>>.
   Proof.
     inv WF1. inv STEP.
@@ -188,7 +187,7 @@ Module Local.
   Lemma silent_step_future lc1 mem1 lc2
         (STEP: silent_step lc1 mem1 lc2)
         (WF1: wf lc1 mem1)
-        (MEM1: Memory.closed mem1):
+        (CLOSED1: Memory.closed mem1):
     wf lc2 mem1.
   Proof.
     inv WF1. inv STEP. ss.
@@ -197,7 +196,7 @@ Module Local.
   Lemma read_step_future lc1 mem1 loc ts val released ord lc2
         (STEP: read_step lc1 mem1 loc ts val released ord lc2)
         (WF1: wf lc1 mem1)
-        (MEM1: Memory.closed mem1):
+        (CLOSED1: Memory.closed mem1):
     wf lc2 mem1.
   Proof.
     inv WF1. inv STEP. econs; ss. apply COMMIT.
@@ -206,7 +205,7 @@ Module Local.
   Lemma fulfill_step_future lc1 mem1 loc from to val releasedc releasedm ord lc2
         (STEP: fulfill_step lc1 mem1 loc from to val releasedc releasedm ord lc2)
         (WF1: wf lc1 mem1)
-        (MEM1: Memory.closed mem1):
+        (CLOSED1: Memory.closed mem1):
     wf lc2 mem1.
   Proof.
     inv WF1. inv STEP. econs; ss.
@@ -217,9 +216,9 @@ Module Local.
   Lemma write_step_future lc1 mem1 loc from to val releasedc releasedm ord lc2 mem2
         (STEP: write_step lc1 mem1 loc from to val releasedc releasedm ord lc2 mem2)
         (WF1: wf lc1 mem1)
-        (MEM1: Memory.closed mem1):
+        (CLOSED1: Memory.closed mem1):
     <<WF2: wf lc2 mem2>> /\
-    <<MEM2: Memory.closed mem2>> /\
+    <<CLOSED2: Memory.closed mem2>> /\
     <<FUTURE: Memory.future mem1 mem2>>.
   Proof.
     inv STEP.
@@ -231,7 +230,7 @@ Module Local.
   Lemma fence_step_future lc1 mem1 ordr ordw lc2
         (STEP: fence_step lc1 mem1 ordr ordw lc2)
         (WF1: wf lc1 mem1)
-        (MEM1: Memory.closed mem1):
+        (CLOSED1: Memory.closed mem1):
     wf lc2 mem1.
   Proof.
     inv WF1. inv STEP. econs; ss. apply WRITE.
@@ -241,7 +240,7 @@ Module Local.
         lc1 mem1 loc from to val released lc2 mem2 lc
         (STEP: promise_step lc1 mem1 loc from to val released lc2 mem2)
         (WF1: wf lc1 mem1)
-        (MEM1: Memory.closed mem1)
+        (CLOSED1: Memory.closed mem1)
         (DISJOINT1: disjoint lc1 lc)
         (WF: wf lc mem1):
     <<DISJOINT2: disjoint lc2 lc>> /\
@@ -279,7 +278,7 @@ Module Local.
         lc1 mem1 lc2 loc from to val releasedc releasedm ord lc
         (STEP: fulfill_step lc1 mem1 loc from to val releasedc releasedm ord lc2)
         (WF1: wf lc1 mem1)
-        (MEM1: Memory.closed mem1)
+        (CLOSED1: Memory.closed mem1)
         (DISJOINT1: disjoint lc1 lc)
         (WF: wf lc mem1):
     disjoint lc2 lc.
@@ -294,7 +293,7 @@ Module Local.
         lc1 mem1 lc2 loc from to val releasedc releasedm ord mem2 lc
         (STEP: write_step lc1 mem1 loc from to val releasedc releasedm ord lc2 mem2)
         (WF1: wf lc1 mem1)
-        (MEM1: Memory.closed mem1)
+        (CLOSED1: Memory.closed mem1)
         (DISJOINT1: disjoint lc1 lc)
         (WF: wf lc mem1):
     <<DISJOINT2: disjoint lc2 lc>> /\
@@ -419,9 +418,9 @@ Module Thread.
           loc from to val released e1 e2
           (STEP: promise_step e1 loc from to val released e2)
           (WF1: Local.wf e1.(local) e1.(memory))
-          (MEM1: Memory.closed e1.(memory)):
+          (CLOSED1: Memory.closed e1.(memory)):
       <<WF2: Local.wf e2.(local) e2.(memory)>> /\
-      <<MEM2: Memory.closed e2.(memory)>> /\
+      <<CLOSED2: Memory.closed e2.(memory)>> /\
       <<FUTURE: Memory.future e1.(memory) e2.(memory)>>.
     Proof.
       inv WF1. inv STEP. s.
@@ -432,9 +431,9 @@ Module Thread.
     Lemma program_step_future e e1 e2
           (STEP: program_step e e1 e2)
           (WF1: Local.wf e1.(local) e1.(memory))
-          (MEM1: Memory.closed e1.(memory)):
+          (CLOSED1: Memory.closed e1.(memory)):
       <<WF2: Local.wf e2.(local) e2.(memory)>> /\
-      <<MEM2: Memory.closed e2.(memory)>> /\
+      <<CLOSED2: Memory.closed e2.(memory)>> /\
       <<FUTURE: Memory.future e1.(memory) e2.(memory)>>.
     Proof.
       inv STEP; ss.
@@ -450,9 +449,9 @@ Module Thread.
     Lemma step_future e e1 e2
           (STEP: step e e1 e2)
           (WF1: Local.wf e1.(local) e1.(memory))
-          (MEM1: Memory.closed e1.(memory)):
+          (CLOSED1: Memory.closed e1.(memory)):
       <<WF2: Local.wf e2.(local) e2.(memory)>> /\
-      <<MEM2: Memory.closed e2.(memory)>> /\
+      <<CLOSED2: Memory.closed e2.(memory)>> /\
       <<FUTURE: Memory.future e1.(memory) e2.(memory)>>.
     Proof.
       inv STEP.
@@ -463,9 +462,9 @@ Module Thread.
     Lemma rtc_step_future e1 e2
           (STEP: rtc tau_step e1 e2)
           (WF1: Local.wf e1.(local) e1.(memory))
-          (MEM1: Memory.closed e1.(memory)):
+          (CLOSED1: Memory.closed e1.(memory)):
       <<WF2: Local.wf e2.(local) e2.(memory)>> /\
-      <<MEM2: Memory.closed e2.(memory)>> /\
+      <<CLOSED2: Memory.closed e2.(memory)>> /\
       <<FUTURE: Memory.future e1.(memory) e2.(memory)>>.
     Proof.
       revert WF1. induction STEP.
@@ -480,7 +479,7 @@ Module Thread.
           loc from to val released e1 e2 lc
         (STEP: promise_step e1 loc from to val released e2)
         (WF1: Local.wf e1.(local) e1.(memory))
-        (MEM1: Memory.closed e1.(memory))
+        (CLOSED1: Memory.closed e1.(memory))
         (DISJOINT1: Local.disjoint e1.(local) lc)
         (WF: Local.wf lc e1.(memory)):
       <<DISJOINT2: Local.disjoint e2.(local) lc>> /\
@@ -494,7 +493,7 @@ Module Thread.
     Lemma program_step_disjoint e e1 e2 lc
         (STEP: program_step e e1 e2)
         (WF1: Local.wf e1.(local) e1.(memory))
-        (MEM1: Memory.closed e1.(memory))
+        (CLOSED1: Memory.closed e1.(memory))
         (DISJOINT1: Local.disjoint e1.(local) lc)
         (WF: Local.wf lc e1.(memory)):
       <<DISJOINT2: Local.disjoint e2.(local) lc>> /\
@@ -520,7 +519,7 @@ Module Thread.
     Lemma step_disjoint e e1 e2 lc
         (STEP: step e e1 e2)
         (WF1: Local.wf e1.(local) e1.(memory))
-        (MEM1: Memory.closed e1.(memory))
+        (CLOSED1: Memory.closed e1.(memory))
         (DISJOINT1: Local.disjoint e1.(local) lc)
         (WF: Local.wf lc e1.(memory)):
       <<DISJOINT2: Local.disjoint e2.(local) lc>> /\
@@ -534,7 +533,7 @@ Module Thread.
     Lemma rtc_step_disjoint e1 e2 lc
         (STEP: rtc tau_step e1 e2)
         (WF1: Local.wf e1.(local) e1.(memory))
-        (MEM1: Memory.closed e1.(memory))
+        (CLOSED1: Memory.closed e1.(memory))
         (DISJOINT1: Local.disjoint e1.(local) lc)
         (WF: Local.wf lc e1.(memory)):
       <<DISJOINT2: Local.disjoint e2.(local) lc>> /\
